Almost finished fundamental theorem proof

theories/STLC.v
@@ -20,17 +20,19 @@ Module STLC.
 
   Definition empty_context : context := fun n => None.
 
-  Definition context_update (c: context) n t := fun m => if Nat.eqb m n then Some t else c m.
-  Notation "X , Y ::: Z" := (context_update X Y Z) (at level 3).
+  Definition context_update (c: context) n t := fun m => if Nat.eqb m n then c m else Some t.
+  Notation "X , Y ::: Z" := (context_update X Y Z) (at level 100).
 
   Notation "∅" := empty_context.
 
-  Inductive typing_derivation : context -> expr -> tipe -> Prop :=
-  | unit_intro: typing_derivation ∅ null unit
-  | axiom_rule Γ (n: name) (t: tipe) (H: Γ n = Some t) : typing_derivation Γ (var n) t
-  | weakening Γ e t n t_var (H: Γ n = None) : typing_derivation Γ e t -> typing_derivation (Γ, n ::: t_var) e t
-  | arrow_elim Γ e1 e2 t_arg t_bod : typing_derivation Γ e1 (arrow t_arg t_bod) -> typing_derivation Γ e2 t_arg -> typing_derivation Γ (app e1 e2) t_bod
-  | arrow_intro Γ n e t_arg t_bod : typing_derivation (Γ, n ::: t_arg) e t_bod -> typing_derivation Γ (abs n e) (arrow t_arg t_bod).
+  Inductive type_checks : context -> expr -> tipe -> Prop :=
+  | unit_intro: type_checks ∅ null unit
+  | axiom_rule Γ (n: name) (t: tipe) (H: Γ n = Some t) : type_checks Γ (var n) t
+  | weakening Γ e t n t_var (H: Γ n = None) : type_checks Γ e t -> type_checks (Γ, n ::: t_var) e t
+  | arrow_elim Γ e1 e2 t_arg t_bod : type_checks Γ e1 (arrow t_arg t_bod) -> type_checks Γ e2 t_arg -> type_checks Γ (app e1 e2) t_bod
+  | arrow_intro Γ n e t_arg t_bod : type_checks (Γ, n ::: t_arg) e t_bod -> type_checks Γ (abs n e) (arrow t_arg t_bod).
+
+  Notation " C ⊢ E ::: T " := (type_checks C E T) (at level 99).
 
   (* Substituition *)
   Fixpoint substitute e1 n e2 : expr :=
@@ -39,6 +41,23 @@ Module STLC.
     | var n' => if Nat.eqb n n' then e2 else e1
     | app e e' => app (substitute e n e2) (substitute e' n e2)
     | abs n' e => if Nat.eqb n n' then e1 else abs n' (substitute e n e2)
+    end.
+
+  (* The type of little gamma *)
+  Definition substitution_maps : Type := name -> option expr.
+
+  Fixpoint parallel_subst e γ : expr :=
+    match e with
+    | null => null
+    | var n =>
+        match (γ n) with
+        | Some e' => e'
+        | None => e
+        end
+    | app e e' => app (parallel_subst e γ) (parallel_subst e' γ)
+    | abs n e =>
+        let γ' := fun m => if Nat.eqb m n then None else γ m in
+        abs n (parallel_subst e γ')
     end.
 
   Inductive is_value : expr -> Prop :=
@@ -74,13 +93,82 @@ Module STLC.
   (*   E : tipe -> expr -> Prop := *)
   (* | E_t t e v (H: is_value v) : cbv_multi e v -> V t v -> E t v. *)
 
-  Program Fixpoint
-    V (t : tipe) : expr -> Prop :=
+  Fixpoint
+    V t v {struct t} : Prop :=
+    let E t e : Prop := exists v, (cbv_multi e v) /\ (V t v) in
     match t with
-    | unit => fun v => true
-    | arrow t1 t2 => fun v => exists e.
-    end
-    and
-    E (t : tipe) : expr -> bool :=
+    | unit => v = null
+    | arrow t1 t2 => exists (n: name) (e: expr), ((v = abs n e) /\ (forall (v': expr), V t1 v' -> E t2 (substitute e n v')))
+    end.
 
+  Definition type_checks_parallel_subst Γ γ : Prop :=
+    forall (n: name), forall t, Γ n = Some t -> exists v, (γ n = Some v) /\ (V t v).
+
+  (* Notation " C ⊨ G " := (type_checks_parallel_subst C G) (at level 99). *)
+
+  Definition type_checks_semantically Γ e t : Prop :=
+    forall γ, (type_checks_parallel_subst Γ γ) -> (exists v, (cbv_multi (parallel_subst e γ) v) /\ (V t v)).
+
+  Notation " C ⊨ E ::: T " := (type_checks_semantically C E T) (at level 99).
+
+  Lemma type_check_parallel_subst_update : forall Γ γ n t,
+       type_checks_parallel_subst (Γ, n ::: t) γ -> type_checks_parallel_subst Γ γ.
+  Proof.
+    unfold type_checks_parallel_subst. intros. specialize H with (n := n0) (t := t0).
+    unfold context_update in H. destruct (Nat.eqb n0 n).
+    - inversion H0. auto.
+    - admit.
+  Admitted.
+
+  Lemma cbv_multi_under_fun : forall e1 e1' e2,
+      cbv_multi e1 e1' -> cbv_multi (app e1 e2) (app e1' e2).
+  Proof.
+    intros. induction H.
+    - apply base_cbv_multi, fun_cbv_once. auto.
+    - apply refl_cbv_multi.
+    - apply (trans_cbv_multi (app e1 e2) (app e0 e2) (app e3 e2)); auto.
+  Qed.
+
+  Lemma cbv_multi_under_arg : forall n e1 e e',
+      cbv_multi e e' -> cbv_multi (app (abs n e1) e) (app (abs n e1) e').
+  Proof.
+    intros. induction H.
+    - apply base_cbv_multi, arg_cbv_once. apply abs_is_value.
+    - apply refl_cbv_multi.
+    - apply (trans_cbv_multi (app (abs n e1) e0) (app (abs n e1) e2) (app (abs n e1) e3)); auto.
+  Qed.
+
+  (* Fundamental theorem of logical relations *)
+  Theorem fundamental_theorem : forall Γ e t, ( Γ ⊢ e ::: t ) -> ( Γ ⊨ e ::: t ).
+  Proof.
+    intros. unfold type_checks_semantically. induction H.
+    - intros. eexists null. split.
+      + simpl. apply refl_cbv_multi.
+      + reflexivity.
+    - intros. simpl. unfold type_checks_parallel_subst in H0. destruct (H0 n t).
+      + apply H.
+      + simpl. destruct H1. rewrite H1. eexists x. split.
+        * apply refl_cbv_multi.
+        * auto.
+    - intros. specialize IHtype_checks with (γ := γ). simpl in H1. apply type_check_parallel_subst_update in H1. auto.
+    - simpl. intros. specialize (IHtype_checks1 γ H1). specialize (IHtype_checks2 γ H1).
+      destruct IHtype_checks1, IHtype_checks2. destruct H2, H3. inversion H4. destruct H6.
+      destruct H6. rewrite H6 in H2. specialize (H7 x0). apply H7 in H5 as H8. clear H7. destruct H8. destruct H7. exists x3. split.
+      + apply (trans_cbv_multi (app (parallel_subst e1 γ) (parallel_subst e2 γ)) (app ((abs x1 x2)) (parallel_subst e2 γ))).
+        * apply cbv_multi_under_fun. auto.
+        * apply trans_cbv_multi with (e2 := (substitute x2 x1 x0)).
+          -- assert (cbv_multi (app (abs x1 x2) (parallel_subst e2 γ)) (app (abs x1 x2) x0)) as Hyp. { apply cbv_multi_under_arg with (e' := x0). auto. } apply trans_cbv_multi with (e2 := (app (abs x1 x2) x0)).
+             ++ auto.
+             ++ apply base_cbv_multi. apply app_cbv_once. unfold V in H5. destruct t_arg.
+                ** subst x0. apply null_is_value.
+                ** destruct H5. destruct H5. destruct H5. subst x0. apply abs_is_value.
+          -- auto.
+      + auto.
+    - intros. specialize (IHtype_checks γ). eexists (parallel_subst (abs n e) γ).
+      split.
+      + apply refl_cbv_multi.
+      + simpl (parallel_subst (abs n e) γ). simpl. eexists n. eexists (parallel_subst e (fun m : nat => if Nat.eqb m n then None else γ m)). split.
+        * reflexivity.
+        * intros. esplit.
+  Admitted.
 End STLC.
